arm+riscv infoflow: remove Kernel_Config.maxIRQ_def instances
By redefining timer_irq as maxIRQ - 1, we avoid using Kernel_Config.maxIRQ_def
in the InfoFlow example state proofs. This exploits the fact that 0 < maxIRQ.

Signed-off-by: Ryan Barry <ryan.barry@proofcraft.systems>

squash infoflow

proof/infoflow/ARM/Example_Valid_State.thy
@@ -27,8 +27,13 @@ consts s0_context :: user_context
 
 (* define the irqs to come regularly every 10 *)
 
+definition timer_irq :: irq where
+  "timer_irq \<equiv> maxIRQ - 1"
+
+abbreviation (input) "timer_int \<equiv> 10"
+
 axiomatization where
-  irq_oracle_def: "ARM.irq_oracle \<equiv> \<lambda>pos. if pos mod 10 = 0 then 10 else 0"
+  irq_oracle_def: "ARM.irq_oracle \<equiv> \<lambda>pos. if pos mod timer_int = 0 then timer_irq else 0"
 
 context begin interpretation Arch . (*FIXME: arch-split*)
 
@@ -219,8 +224,6 @@ definition "Silc_cnode_ptr = init_objs_base + 0x18000"
 definition "irq_cnode_ptr = init_objs_base + 0x1C000"
 
 (* init_global_pd \<equiv> {init_objs_base + 0x60000,... init_objs_base + 0x603555} *)
-
-definition "timer_irq \<equiv> 10" (* not sure exactly how this fits in *)
 
 definition "Low_mcp \<equiv> 5 :: word8"
 definition "Low_prio \<equiv> 5 :: word8"
@@ -1155,12 +1158,12 @@ lemma silc_inv_s0:
   apply (clarsimp simp: Invariants_AI.cte_wp_at_caps_of_state )
   by (auto simp:is_transferable.simps dest:s0_caps_of_state)
 
-
 lemma only_timer_irq_s0:
   "only_timer_irq timer_irq s0_internal"
   apply (clarsimp simp: only_timer_irq_def s0_internal_def irq_is_recurring_def is_irq_at_def
                         irq_at_def Let_def irq_oracle_def machine_state0_def timer_irq_def)
-  apply presburger
+  apply (erule_tac x="timer_int - n mod timer_int" in allE)
+  apply (subst (asm) mod_add_left_eq[symmetric], simp)
   done
 
 lemma domain_sep_inv_s0:
