proof/infoflow/refine/RISCV64/Example_Valid_StateH.thy
@@ -3239,6 +3239,14 @@ lemma valid_arch_state_s0H:
   apply (clarsimp simp: arch_state0H_def)
   done
 
+lemma timer_irq_not_outside_range[simp]:
+  "\<not> maxIRQ < timer_irq"
+  apply (simp add: timer_irq_def)
+  apply (rule leD)
+  apply (rule word_sub_1_le)
+  apply (simp add: word_neq_0_conv maxIRQ_def)
+  done
+
 lemma s0H_invs:
   assumes "1 \<le> maxDomain"
   notes pteBits_def[simp] objBits_defs[simp]
@@ -3416,7 +3424,7 @@ lemma s0H_invs:
   apply (rule conjI)
    apply (clarsimp simp: valid_machine_state'_def s0H_internal_def machine_state0_def)
   apply (rule conjI)
-   apply (clarsimp simp: irqs_masked'_def s0H_internal_def maxIRQ_def timer_irq_def irqInvalid_def)
+   apply (clarsimp simp: irqs_masked'_def s0H_internal_def irqInvalid_def)
   apply (rule conjI)
    apply (clarsimp simp: sym_heap_def opt_map_def projectKOs split: option.splits)
    using kh0H_dom_tcb
